theories/compiler/numbers.v
@@ -47,10 +47,10 @@ Definition compile_sign (s : rwasm.Sign) : wasm.sx :=
   | rwasm.S => wasm.SX_S
   end.
 
-Definition throw_missing (instr_name : string) : M wasm.basic_instruction :=
-  mthrow (err ("missing iris-wasm " ++ instr_name ++ " wrap instruction")).
+Definition throw_missing (instr_name : string) : exn err wasm.basic_instruction :=
+  mthrow (Err ("missing iris-wasm " ++ instr_name ++ " wrap instruction")).
 
-Definition compile_num_intr (ni : rwasm.NumInstr) : M wasm.basic_instruction :=
+Definition compile_num_intr (ni : rwasm.NumInstr) : exn err wasm.basic_instruction :=
   match ni with
   | rwasm.Iu typ op =>
     let typ' := compile_int_type typ in
